SSA/Experimental/Bits/Fast/Decide.lean
@@ -4,7 +4,9 @@ import SSA.Experimental.Bits.Fast.Lemmas
 instance (t₁ t₂ : Term) : Decidable (t₁.eval = t₂.eval) :=
   decidable_of_iff
     (decideIfZeros (termEvalEqFSM (t₁.xor t₂)).toFSM) $ by
-  rw [decideIfZeros_correct, ← (termEvalEqFSM (t₁.xor t₂)).good]
+  rw [decideIfZeros_correct]
+  simp only [eval_simplify]
+  rw [← (termEvalEqFSM (t₁.xor t₂)).good]
   simp only [eval_eq_iff_xor_eq_zero]
   rw [forall_swap]
   simp only [← funext_iff]
@@ -13,7 +15,9 @@ instance (p : Predicate) :
     Decidable (∀ (n : ℕ) (x : Fin p.arity → BitStream) , p.evalFin x n = false) :=
   decidable_of_iff
     (decideIfZeros (predicateEvalEqFSM p).toFSM) $ by
-  rw [decideIfZeros_correct, ← (predicateEvalEqFSM p).good]
+  rw [decideIfZeros_correct]
+  simp only [eval_simplify]
+  rw [← (predicateEvalEqFSM p).good]
 
 /--
 We can decide that the evaluation of a predicate is forever false,
@@ -23,7 +27,9 @@ instance (p : Predicate) :
     Decidable (∀ (n : ℕ) (x : List BitStream) , p.eval x n = false) :=
   decidable_of_iff
     (decideIfZeros (predicateEvalEqFSM p).toFSM) $ by
-  rw [decideIfZeros_correct, ← (predicateEvalEqFSM p).good]
+  rw [decideIfZeros_correct]
+  simp only [eval_simplify]
+  rw [← (predicateEvalEqFSM p).good]
   constructor <;> sorry
 
 instance (p : Predicate) (n : ℕ) : 
